src/Noninterference/RefinesSame.v
@@ -1,0 +1,304 @@
+Require Import Framework File FileDiskLayer FileDiskNoninterference FileDiskRefinement.
+Require Import FunctionalExtensionality Lia.
+Require Import AuthenticationLayer TransactionalDiskLayer AuthenticatedDiskLayer.
+
+Lemma exec_Crash_finished_exfalso:
+forall O (L: Language O) u T (p: L.(prog) T) s s' r,
+~exec L u [Language.Crash O] s p (Finished s' r).
+Proof.
+    unfold not; induction p; simpl; intros;
+    invert_exec.
+    symmetry in H2; apply app_eq_unit in H2;
+    intuition cleanup;
+    exfalso; eapply exec_empty_oracle; eauto.
+Qed.
+
+Lemma exec_finished_no_crash_tokens:
+forall u T (p: Definitions.impl.(prog) T) o s s' r,
+exec Definitions.impl u o s p (Finished s' r) -> 
+(forall (t: Definitions.impl.(token)), In t o -> 
+t <> Language.Crash _ /\ 
+t <> OpToken AuthenticatedDiskOperation (Token1 AuthenticationOperation _ Crash) /\
+t <> OpToken AuthenticatedDiskOperation (Token2 _ (TransactionalDiskOperation FSParameters.data_length) CrashBefore) /\
+t <> OpToken AuthenticatedDiskOperation (Token2 _ (TransactionalDiskOperation FSParameters.data_length) CrashAfter) /\
+t <> OpToken AuthenticatedDiskOperation (Token2 _ (TransactionalDiskOperation FSParameters.data_length) CrashDuringCommit)).
+Proof.
+    induction p; simpl; intros;
+    invert_exec.
+    {
+        destruct o; invert_exec;
+        destruct o; invert_exec;
+        (inversion H0; cleanup;
+        [ repeat (split; try congruence)
+        | inversion H]).
+    }
+    {
+        inversion H0; cleanup;
+        [ repeat (split; try congruence)
+        | inversion H].
+    }
+    {
+        eapply in_app_iff in H1; split_ors; eauto.
+    }
+Qed.   
+
+Lemma exec_crashed_exists_crash_token:
+forall u T (p: Definitions.impl.(prog) T) o s s',
+exec Definitions.impl u o s p (Crashed s') -> 
+(exists (t: Definitions.impl.(token)), 
+In t o /\
+( 
+t = Language.Crash _ \/
+t = OpToken AuthenticatedDiskOperation (Token1 AuthenticationOperation _ Crash) \/
+t = OpToken AuthenticatedDiskOperation (Token2 _ (TransactionalDiskOperation FSParameters.data_length) CrashBefore) \/
+t = OpToken AuthenticatedDiskOperation (Token2 _ (TransactionalDiskOperation FSParameters.data_length) CrashAfter) \/
+t = OpToken AuthenticatedDiskOperation (Token2 _ (TransactionalDiskOperation FSParameters.data_length) CrashDuringCommit))
+).
+Proof.
+    induction p; simpl; intros;
+    invert_exec.
+    {
+        destruct o; invert_exec;
+        destruct o; invert_exec.
+        all: eexists; split; [econstructor; eauto | eauto].
+    }
+    {
+        eexists; split; [econstructor; eauto | eauto].
+    }
+    {
+        split_ors; cleanup.
+        edestruct IHp; eauto.
+        cleanup.
+        eexists; split.
+        apply in_app_iff; eauto.
+        eauto.
+
+        edestruct H; eauto.
+        cleanup.
+        eexists; split.
+        apply in_app_iff; eauto.
+        eauto.
+    }
+Qed.   
+
+Lemma exec_finished_not_crashed:
+forall u T (p: Definitions.impl.(prog) T) o s s' s1 s1' r,
+exec Definitions.impl u o s p (Finished s' r) -> 
+~exec Definitions.impl u o s1 p (Crashed s1').
+Proof.
+  unfold not; intros.
+  eapply exec_crashed_exists_crash_token in H0; cleanup.
+  eapply exec_finished_no_crash_tokens in H; eauto.
+  cleanup; intuition; subst; congruence.
+Qed.
+
+Lemma token_refines_same_read:
+forall u u' o_imp s1_imp s2_imp x x0  get_reboot_state 
+o_abs o_abs' inum off,
+    refines s1_imp x ->
+    refines s2_imp x0 ->
+    same_for_user_except u' None x x0 ->
+    oracle_refines _ _ _ Definitions.abs FileDiskOperationRefinement _ u s1_imp 
+    (|Read inum off|) get_reboot_state  o_imp o_abs ->
+    oracle_refines _ _ _ Definitions.abs FileDiskOperationRefinement _ u s2_imp 
+    (|Read inum off|) get_reboot_state  o_imp o_abs' ->
+    o_abs = o_abs'.
+Proof.
+    simpl; intros; cleanup.
+    specialize H5 with (1:= H);
+    specialize H4 with (1:= H0);
+    repeat split_ors; cleanup; 
+    repeat unify_execs; eauto.
+    eapply SSERead 
+    unfold read in H3.
+    Search Finished Crashed.
+    edestruct read_simulation; simpl. 
+    2: apply H.
+    2: instantiate (4:=0).
+
+
+
+(*
+Lemma oracle_refines_same:
+forall u u' T (p1 p2: Definitions.abs.(prog) T) s1_imp s2_imp x x0 o_imp o_abs o_abs' get_reboot_state,
+    (forall t t' T (p1 p2: Definitions.abs_core.(operation) T),
+    refines s1_imp x ->
+    refines s2_imp x0 ->
+    same_for_user_except u' None x x0 ->
+    token_refines _ u s1_imp  
+    p1 get_reboot_state  o_imp t ->
+    token_refines _ u s2_imp   
+    p2 get_reboot_state o_imp t' ->
+    t = t') ->
+    refines s1_imp x ->
+    refines s2_imp x0 ->
+    same_for_user_except u' None x x0 ->
+    oracle_refines _ _ _ Definitions.abs FileDiskOperationRefinement _ u s1_imp 
+    p1 get_reboot_state  o_imp o_abs ->
+    oracle_refines _ _ _ Definitions.abs FileDiskOperationRefinement _ u s2_imp 
+    p2 get_reboot_state  o_imp o_abs' ->
+    o_abs = o_abs'.
+    Proof.
+    induction p1; simpl; intros; eauto.
+    {
+        cleanup.
+        destruct p2; simpl in *; cleanup.
+        erewrite H with (t:= x1)(t':=x2); eauto.
+        split_ors; cleanup.
+
+        invert_exec; simpl in *.
+        {
+            unfold refines, files_rep, files_reboot_rep in *.
+            destruct o. 
+            {
+                simpl in *; 
+                unfold refines, files_rep, files_reboot_rep in *;
+                cleanup;
+                edestruct H5; cleanup; eauto; try congruence.
+                split; eauto.
+                setoid_rewrite H0; eauto.
+                exfalso; eapply exec_Crash_finished_exfalso in H6; eauto.
+                
+                unfold read, auth_then_exec in *; simpl in *.
+                invert_exec.
+                symmetry in H10; apply app_eq_unit in H10;
+                intuition cleanup.
+                exfalso; eapply exec_empty_oracle; eauto.
+                Transparent Inode.get_owner.
+                unfold Inode.get_owner in *.
+                invert_exec.
+                destruct x1; simpl in *; try congruence.
+                destruct t; simpl in *; try congruence.
+                invert_exec'' H11.
+                destruct o1.
+                exfalso; eapply exec_empty_oracle; eauto.
+                rewrite <- app_comm_cons in H12.
+                inversion H12; subst.
+                unfold Inode.get_inode, Inode.InodeAllocator.read in *.
+                invert_step.
+        }
+         eauto.
+    }
+    cleanup; simpl in *; try tauto; try lia.
+    repeat split_ors; cleanup;
+    repeat unify_execs; cleanup; try tauto.
+    eapply H in H10; eauto; subst; eauto.
+Qed.
+*)
+
+Lemma recovery_oracles_refine_to_same:
+         forall l_o_imp l_o_abs l_o_abs' s1_imp s2_imp x x0 u u' T (p1 p2: Definitions.abs.(prog) T),
+         (forall o_imp o_abs o_abs' get_reboot_state,
+         refines s1_imp x ->
+            refines s2_imp x0 ->
+        same_for_user_except u' None x x0 ->
+        oracle_refines _ _ _ _ FileDiskOperationRefinement _ u s1_imp 
+        p1 get_reboot_state  o_imp o_abs ->
+        oracle_refines _ _ _ _ FileDiskOperationRefinement _ u s2_imp 
+        p2 get_reboot_state  o_imp o_abs' ->
+            o_abs = o_abs') ->
+         
+         refines s1_imp x ->
+            refines s2_imp x0 ->
+        same_for_user_except u' None x x0 ->
+        recovery_oracles_refine_to FileDiskRefinement u s1_imp p1 
+          (| Recover |) [] l_o_imp l_o_abs ->
+        recovery_oracles_refine_to FileDiskRefinement u s2_imp p2
+            (| Recover |) [] l_o_imp l_o_abs' ->
+       l_o_abs = l_o_abs'.
+       Proof.
+           induction l_o_imp; simpl; intros; try tauto.
+         cleanup; simpl in *; try tauto; try lia.
+         repeat split_ors; cleanup;
+         repeat unify_execs; cleanup; try tauto.
+         eapply H in H10; eauto; subst; eauto.
+       Qed.
+
+       
+
+Lemma ORS_recover:
+forall u u' ex n,
+oracle_refines_same_from_related FileDiskRefinement u 
+(|Recover|)  (|Recover|) (|Recover|) 
+(authenticated_disk_reboot_list n) (same_for_user_except u' ex).
+Proof.
+unfold oracle_refines_same_from_related,
+refines_related.
+    induction n;
+    simpl; intros; cleanup.
+    {
+        destruct l_o_imp; simpl in *; cleanup; eauto; try tauto.
+        repeat split_ors; cleanup; 
+        try unify_execs; cleanup; try tauto.
+        
+        edestruct H13; edestruct H9.
+        all: try solve [unfold refines,
+        files_rep, files_reboot_rep in*;
+        cleanup; simpl; eauto];
+        cleanup; repeat unify_execs; cleanup.
+    }
+    {
+    destruct l_o_imp; simpl in *; cleanup; eauto; try tauto.
+    repeat split_ors; cleanup; 
+    try unify_execs; cleanup; try tauto;
+    simpl in *; try lia.
+    
+    edestruct H13; edestruct H9.
+    all: try solve [unfold refines,
+    files_rep, files_reboot_rep in*;
+    cleanup; simpl; eauto];
+    cleanup; repeat unify_execs; cleanup.
+
+    edestruct H11; edestruct H8.
+    all: try solve [unfold refines,
+    files_rep, files_reboot_rep in*;
+    cleanup; simpl; eauto];
+    cleanup; repeat unify_execs; cleanup.
+
+    erewrite IHn with (l_o_abs := l0) (l_o_abs' := l). 
+    eauto.
+    2: eauto.
+    2: eauto.
+    do 2 eexists. unfold refines, files_rep, files_crash_rep in *.
+    repeat (split; eauto).
+    }
+Qed.
+
+Lemma ORS_read:
+forall u u' inum n off,
+oracle_refines_same_from_related FileDiskRefinement u 
+(|Read inum off|) (|Read inum off|) (|Recover|) 
+(authenticated_disk_reboot_list n) (same_for_user_except u' None).
+Proof.
+    unfold oracle_refines_same_from_related,
+    refines_related; intros; destruct n; simpl in *; cleanup.
+     {
+         eapply recovery_oracles_refine_to_same; [| | |eauto| |]; eauto.
+        (*Oracles refine same*)
+        admit.
+     }
+     {
+         destruct l_o_imp; simpl in *; try tauto.
+         cleanup; try tauto.
+         repeat split_ors; cleanup; 
+         repeat unify_execs; cleanup;
+         simpl in *; try lia.
+
+         eapply_fresh H13 in H;
+         eapply_fresh H9 in H2;
+         clear H9 H13;
+         cleanup; repeat split_ors; cleanup;
+         repeat unify_execs; cleanup; eauto.
+
+         eapply_fresh H11 in H;
+         eapply_fresh H8 in H2;
+         clear H8 H11;
+         cleanup; repeat split_ors; cleanup;
+         repeat unify_execs; cleanup; eauto.
+         erewrite ORS_recover with (l_o_abs := l0) (l_o_abs':= l); eauto.
+         unfold refines_related; simpl.
+         do 2 eexists. 
+         unfold refines, files_rep, files_crash_rep in *.
+        repeat (split; eauto).
+     }
+Admitted.
