src/Noninterference/SSECommon.v
@@ -1,0 +1,1114 @@
+Require Import Framework File FileDiskLayer FileDiskNoninterference FileDiskRefinement.
+Require Import FunctionalExtensionality Lia Language.
+
+Definition AD_valid_state := refines_valid FileDiskRefinement FD_valid_state.
+Definition AD_related_states u exc := refines_related FileDiskRefinement (FD_related_states u exc).
+
+
+Ltac econstructor_recovery :=
+  match goal with
+  | [|- recovery_exec _ ?u [?o] _ [] _ _ _ ]=>
+    eapply (@ExecFinished _ _ _ _ u o)
+  | [|- recovery_exec _ ?u (?o :: _) _ (?rf :: _) _ _ _ ]=>
+    eapply (@ExecRecovered _ _ _ _ u o _ _ _ rf)
+  end.
+
+  Ltac invert_exec_lift_no_match :=
+  match goal with
+  | [H: Language.exec' _ _ _ (Op _ (P1 _)) _ |- _ ]=>
+    invert_exec'' H
+  | [H: Language.exec' _ _ _ (Op _ (P2 _)) _ |- _ ]=>
+    invert_exec'' H
+  | [H: Language.exec' _ _ _ (_ <- lift_L1 _ _; _) _ |- _ ]=>
+    invert_exec'' H
+  | [H: Language.exec' _ _ _ (_ <- lift_L2 _ _; _) _ |- _ ]=>
+    invert_exec'' H
+  | [H: Language.exec' _ _ _ (_ <- Op _ (P1 _); _) _ |- _ ]=>
+    invert_exec'' H
+  | [H: Language.exec' _ _ _ (_ <- Op _ (P2 _); _) _ |- _ ]=>
+    invert_exec'' H
+  | _ =>
+    try invert_exec_no_match
+  end.
+
+  Ltac invert_exec_lift :=
+  match goal with
+  | [H: Language.exec' _ _ _ (Op _ (P1 _)) _ |- _ ]=>
+    invert_exec'' H
+  | [H: Language.exec' _ _ _ (Op _ (P2 _)) _ |- _ ]=>
+    invert_exec'' H
+  | [H: Language.exec' _ _ _ (_ <- lift_L1 _ _; _) _ |- _ ]=>
+    invert_exec'' H
+  | [H: Language.exec' _ _ _ (_ <- lift_L2 _ _; _) _ |- _ ]=>
+    invert_exec'' H
+  | [H: Language.exec' _ _ _ (_ <- Op _ (P1 _); _) _ |- _ ]=>
+    invert_exec'' H
+  | [H: Language.exec' _ _ _ (_ <- Op _ (P2 _); _) _ |- _ ]=>
+    invert_exec'' H
+  | _ =>
+    try invert_exec
+  end.
+
+Theorem SelfSimulation_Exists_recover:
+  forall u n,
+      SelfSimulation_Exists u recover recover recover
+                            AD_valid_state (AD_related_states u None)
+                            (authenticated_disk_reboot_list n).
+Proof.
+  induction n; simpl;
+  unfold SelfSimulation_Exists, AD_valid_state,
+  AD_related_states, FD_valid_state, FD_related_states,
+  refines_valid, refines_related,
+  authenticated_disk_reboot_list in *;
+  intros; cleanup; simpl in *.
+  {
+    invert_exec; cleanup.
+    unfold recover in *; repeat invert_exec; simpl in *.
+    simpl in H11.
+    repeat invert_exec_lift_no_match.
+    eexists.    
+    econstructor_recovery.
+    repeat econstructor.
+  }
+  {
+    invert_exec; cleanup.
+    unfold recover in *; repeat invert_exec; simpl in *.
+    repeat invert_exec_lift_no_match.
+    repeat cleanup_pairs.    
+    destruct s2, s1; simpl in *.
+    edestruct IHn.
+    3: apply H15.
+    intros; eauto.
+    intros; eauto.    
+    instantiate (1:= (s0, (t2, t2))).
+    unfold refines, files_rep in *; simpl in *.
+    cleanup; do 2 eexists; intuition eauto.
+    eexists.
+    econstructor_recovery.
+    repeat econstructor; eauto.
+    simpl; eauto.
+  }
+Qed.
+
+Ltac invert_bind :=
+match goal with
+|[H: exec' _ _ _ (Ret _) _ |- _] =>
+invert_exec'' H
+|[H: exec' _ _ _ (Op _ (P1 _)) _ |- _] =>
+invert_exec'' H
+|[H: exec' _ _ _ (Op _ (P2 _)) _ |- _] =>
+invert_exec'' H
+|[H: exec' _ _ _ (_ <- _ ; _) _ |- _] =>
+invert_exec'' H
+| _ =>
+  try invert_exec
+end.
+
+Ltac invert_bind_no_match :=
+match goal with
+|[H: exec' _ _ _ (Ret _) _ |- _] =>
+invert_exec'' H
+|[H: exec' _ _ _ (Op _ (P1 _)) _ |- _] =>
+invert_exec'' H
+|[H: exec' _ _ _ (Op _ (P2 _)) _ |- _] =>
+invert_exec'' H
+|[H: exec' _ _ _ (_ <- _ ; _) _ |- _] =>
+invert_exec'' H
+| _ =>
+  try invert_exec_no_match
+end.
+
+Set Nested Proofs Allowed.
+Lemma lt_le_lt:
+      forall n m p q,
+      n + m < q -> p <= m -> n + p < q.
+Proof.  lia. Qed.
+
+Lemma nth_error_None_r :
+forall T (l: list T) n,
+n >= length l ->
+nth_error l n = None.
+Proof.
+  apply nth_error_None.
+Qed.
+
+Lemma bind_reorder_l:
+  forall O (L: Language O) T  
+  (p1: prog L T) T' (p2: T -> prog L T') 
+  T'' (p3: T' -> prog L T'') 
+  u o s r,
+      exec L u o s (Bind p1 (fun t => Bind (p2 t) p3)) r ->
+      exec L u o s (Bind (Bind p1 p2) p3) r.
+Proof.  Proof.
+eapply bind_reorder.
+Qed.
+
+Lemma bind_reorder_r:
+  forall O (L: Language O) T  
+  (p1: prog L T) T' (p2: T -> prog L T') 
+  T'' (p3: T' -> prog L T'') 
+  u o s r,
+  exec L u o s (Bind (Bind p1 p2) p3) r ->
+      exec L u o s (Bind p1 (fun t => Bind (p2 t) p3)) r.
+      
+Proof.  Proof.
+eapply bind_reorder.
+Qed.
+
+Lemma inode_allocations_are_same:
+forall u fm1 fm2 s1 s2 t1 t2 inum ex,
+refines s1 fm1 ->
+refines s2 fm2 ->
+same_for_user_except u ex fm1 fm2 ->
+inum < Inode.InodeAllocatorParams.num_of_blocks ->
+t1 = fst (snd s1) ->
+t2 = fst (snd s2) ->
+nth_error
+(value_to_bits
+  (t1 Inode.InodeAllocatorParams.bitmap_addr))
+inum =
+nth_error
+  (value_to_bits (t2 
+  Inode.InodeAllocatorParams.bitmap_addr)) inum.
+Proof.
+  unfold refines, files_rep, 
+  files_inner_rep, same_for_user_except; intros.
+  cleanup; repeat cleanup_pairs.
+  destruct_fresh (x inum).
+  {
+    eapply_fresh FileInnerSpecs.inode_exists_then_file_exists in D; eauto.
+    cleanup.
+    destruct_fresh (fm1 inum).
+    {
+      destruct_fresh (x1 inum).
+      unfold Inode.inode_rep, 
+      Inode.inode_map_rep,
+      Inode.InodeAllocator.block_allocator_rep in *.
+      cleanup.
+      eapply Inode.InodeAllocator.valid_bits_extract with (n:= inum) in H10.
+      cleanup; split_ors; cleanup; try congruence.
+      rewrite H4, H10 in D; simpl in *; congruence.
+      rewrite nth_seln_eq in H3.
+      repeat erewrite nth_error_nth'.
+
+      eapply Inode.InodeAllocator.valid_bits_extract with (n:= inum) in H17.
+      cleanup; split_ors; cleanup; try congruence.
+      rewrite H15, H21 in D1; simpl in *; congruence.
+      rewrite nth_seln_eq in H20.
+      rewrite H3, H20; eauto.
+      all: try rewrite value_to_bits_length;
+      unfold Inode.InodeAllocatorParams.num_of_blocks in *;
+      pose proof Inode.InodeAllocatorParams.num_of_blocks_in_bounds; try lia.
+
+      unfold file_map_rep in *; cleanup.
+      edestruct H9; exfalso.
+      apply H13; eauto; congruence.
+    }
+    {
+      edestruct H1; exfalso.
+      apply H3; eauto; congruence.
+    }
+  }
+  {
+    eapply_fresh FileInnerSpecs.inode_missing_then_file_missing in D; eauto.
+    cleanup.
+    destruct_fresh (fm1 inum).
+    {
+      edestruct H1; exfalso.
+      apply H; eauto; congruence.
+    }
+    destruct_fresh (x1 inum).
+    {
+      unfold file_map_rep in *; cleanup.
+      edestruct H3; exfalso.
+      apply H12; eauto; congruence.
+    }
+    {
+      unfold Inode.inode_rep, 
+      Inode.inode_map_rep,
+      Inode.InodeAllocator.block_allocator_rep in *.
+      cleanup.
+      eapply Inode.InodeAllocator.valid_bits_extract with (n:= inum) in H7.
+      cleanup; split_ors; cleanup; try congruence.
+      rewrite nth_seln_eq in H0.
+      repeat erewrite nth_error_nth'.
+
+      eapply Inode.InodeAllocator.valid_bits_extract with (n:= inum) in H16.
+      cleanup; split_ors; cleanup; try congruence.
+      rewrite nth_seln_eq in H19.
+      rewrite H0, H19; eauto.
+      rewrite H14, H20 in D1; simpl in *; congruence.
+      all: try rewrite value_to_bits_length;
+      unfold Inode.InodeAllocatorParams.num_of_blocks in *;
+      pose proof Inode.InodeAllocatorParams.num_of_blocks_in_bounds; try lia.
+      rewrite H3, H7 in D; simpl in *; congruence.
+    }
+  }
+Qed.
+
+Lemma inode_owners_are_same:
+forall u fm1 fm2 s1 s2 t1 t2 inum ex,
+refines s1 fm1 ->
+refines s2 fm2 ->
+same_for_user_except u ex fm1 fm2 ->
+inum < Inode.InodeAllocatorParams.num_of_blocks ->
+nth_error
+(value_to_bits
+  (t1 Inode.InodeAllocatorParams.bitmap_addr))
+inum = Some true ->
+t1 = fst (snd s1) ->
+t2 = fst (snd s2) ->
+  Inode.owner (Inode.decode_inode
+(t1 (Inode.InodeAllocatorParams.bitmap_addr + S inum))) =
+  Inode.owner
+(Inode.decode_inode
+(t2 (Inode.InodeAllocatorParams.bitmap_addr + S inum))).
+Proof.
+  unfold refines, files_rep, 
+  files_inner_rep, same_for_user_except; intros.
+  cleanup; repeat cleanup_pairs.
+  destruct_fresh (x1 inum).
+  {
+    eapply_fresh FileInnerSpecs.inode_exists_then_file_exists in D; eauto.
+    cleanup.
+    destruct_fresh (fm2 inum).
+    {
+      destruct_fresh (x inum).
+      eapply_fresh H7 in D0; eauto; cleanup.
+      unfold file_map_rep in *; cleanup.
+      eapply_fresh H10 in D0; eauto.
+      eapply_fresh H14 in D; eauto.
+      unfold file_rep in *; cleanup.
+
+      unfold Inode.inode_rep, 
+      Inode.inode_map_rep,
+      Inode.InodeAllocator.block_allocator_rep in *.
+      cleanup.
+      eapply Inode.InodeAllocator.valid_bits_extract with (n:= inum) in H23.
+      cleanup; split_ors; cleanup; try congruence.
+      rewrite H21, H23 in D1; simpl in *; congruence.
+      rewrite H21, H23 in D1; simpl in *.
+      cleanup.
+
+      eapply Inode.InodeAllocator.valid_bits_extract with (n:= inum) in H28.
+      cleanup; split_ors; cleanup; try congruence.
+      rewrite H26, H32 in D; simpl in *; congruence.
+      rewrite H26, H32 in D; simpl in *; cleanup.
+      eauto.
+
+      all: try rewrite value_to_bits_length;
+      unfold Inode.InodeAllocatorParams.num_of_blocks in *;
+      pose proof Inode.InodeAllocatorParams.num_of_blocks_in_bounds; try lia.
+
+      unfold file_map_rep in *; cleanup.
+      edestruct H4; exfalso.
+      apply H14; eauto; congruence.
+    }
+    {
+      edestruct H1; exfalso.
+      apply H0; eauto; congruence.
+    }
+  }
+  {
+    unfold Inode.inode_rep, 
+      Inode.inode_map_rep,
+      Inode.InodeAllocator.block_allocator_rep in *.
+      cleanup.
+      eapply Inode.InodeAllocator.valid_bits_extract with (n:= inum) in H17.
+      cleanup; split_ors; cleanup; try congruence.
+      eapply nth_error_nth in H3.
+      rewrite <- nth_seln_eq in H3.
+      rewrite H0 in H3; congruence.
+      rewrite H15, H17 in D; simpl in *; congruence.
+
+      all: try rewrite value_to_bits_length;
+      unfold Inode.InodeAllocatorParams.num_of_blocks in *;
+      pose proof Inode.InodeAllocatorParams.num_of_blocks_in_bounds; try lia.
+  }
+Qed.
+
+
+Lemma block_numbers_in_length:
+forall inum off a s2 d' x x0 u ex,
+refines d' x ->
+refines s2 x0 ->
+same_for_user_except u ex x x0 ->
+inum < Inode.InodeAllocatorParams.num_of_blocks ->
+nth_error
+(value_to_bits
+  (fst (snd d') Inode.InodeAllocatorParams.bitmap_addr))
+inum = Some true ->
+nth_error
+ (Inode.block_numbers
+    (Inode.decode_inode
+       (fst (snd d') (Inode.InodeAllocatorParams.bitmap_addr + S inum))))
+ off = Some a ->
+off <
+length
+(Inode.block_numbers
+(Inode.decode_inode
+  (fst (snd s2)
+     (Inode.InodeAllocatorParams.bitmap_addr + S inum)))).
+Proof.
+  unfold refines, files_rep, 
+  files_inner_rep, same_for_user_except; intros.
+  cleanup; repeat cleanup_pairs.
+  destruct_fresh (x3 inum).
+  {
+    eapply_fresh FileInnerSpecs.inode_exists_then_file_exists in D; eauto.
+    cleanup.
+    destruct_fresh (x0 inum).
+    {
+      destruct_fresh (x1 inum).
+      eapply_fresh H6 in D0; eauto; cleanup.
+      unfold file_map_rep in *; cleanup.
+      eapply_fresh H14 in D0; eauto.
+      eapply_fresh H15 in D; eauto.
+      unfold file_rep in *; cleanup.
+
+      unfold Inode.inode_rep, 
+      Inode.inode_map_rep,
+      Inode.InodeAllocator.block_allocator_rep in *.
+      cleanup.
+      eapply Inode.InodeAllocator.valid_bits_extract with (n:= inum) in H24.
+      cleanup; split_ors; cleanup; try congruence.
+      rewrite H22, H24 in D1; simpl in *; congruence.
+      rewrite H22, H24 in D1; simpl in *.
+      cleanup.
+
+      eapply Inode.InodeAllocator.valid_bits_extract with (n:= inum) in H29.
+      cleanup; split_ors; cleanup; try congruence.
+      rewrite H27, H33 in D; simpl in *; congruence.
+      rewrite H27, H33 in D; simpl in *; cleanup.
+      eapply nth_error_Some; eauto; congruence.
+
+      all: try rewrite value_to_bits_length;
+      unfold Inode.InodeAllocatorParams.num_of_blocks in *;
+      pose proof Inode.InodeAllocatorParams.num_of_blocks_in_bounds; try lia.
+
+      unfold file_map_rep in *; cleanup.
+      edestruct H9; exfalso.
+      apply H15; eauto; congruence.
+    }
+    {
+      edestruct H1; exfalso.
+      apply H0; eauto; congruence.
+    }
+  }
+  {
+    unfold Inode.inode_rep, 
+      Inode.inode_map_rep,
+      Inode.InodeAllocator.block_allocator_rep in *.
+      cleanup.
+      eapply Inode.InodeAllocator.valid_bits_extract with (n:= inum) in H18.
+      cleanup; split_ors; cleanup; try congruence.
+      eapply nth_error_nth in H3.
+      rewrite <- nth_seln_eq in H3.
+      rewrite H0 in H3; congruence.
+      rewrite H16, H18 in D; simpl in *; congruence.
+
+      all: try rewrite value_to_bits_length;
+      unfold Inode.InodeAllocatorParams.num_of_blocks in *;
+      pose proof Inode.InodeAllocatorParams.num_of_blocks_in_bounds; try lia.
+  }
+Qed.
+
+Lemma block_numbers_oob:
+forall inum off s2 d' x x0 u,
+refines d' x ->
+refines s2 x0 ->
+same_for_user_except u None x x0 ->
+inum < Inode.InodeAllocatorParams.num_of_blocks ->
+nth_error
+(value_to_bits
+  (fst (snd d') Inode.InodeAllocatorParams.bitmap_addr))
+inum = Some true ->
+nth_error
+ (Inode.block_numbers
+    (Inode.decode_inode
+       (fst (snd d') (Inode.InodeAllocatorParams.bitmap_addr + S inum))))
+ off = None ->
+off >=
+length
+(Inode.block_numbers
+(Inode.decode_inode
+  (fst (snd s2)
+     (Inode.InodeAllocatorParams.bitmap_addr + S inum)))).
+     Proof.
+      unfold refines, files_rep, 
+      files_inner_rep, same_for_user_except; intros.
+      cleanup; repeat cleanup_pairs.
+      destruct_fresh (x3 inum).
+      {
+        eapply_fresh FileInnerSpecs.inode_exists_then_file_exists in D; eauto.
+        cleanup.
+        destruct_fresh (x0 inum).
+        {
+          destruct_fresh (x1 inum).
+          eapply_fresh H6 in D0; eauto; cleanup.
+          unfold file_map_rep in *; cleanup.
+          eapply_fresh H14 in D0; eauto.
+          eapply_fresh H15 in D; eauto.
+          unfold file_rep in *; cleanup.
+    
+          unfold Inode.inode_rep, 
+          Inode.inode_map_rep,
+          Inode.InodeAllocator.block_allocator_rep in *.
+          cleanup.
+          eapply Inode.InodeAllocator.valid_bits_extract with (n:= inum) in H24.
+          cleanup; split_ors; cleanup; try congruence.
+          rewrite H22, H24 in D1; simpl in *; congruence.
+          rewrite H22, H24 in D1; simpl in *.
+          cleanup.
+    
+          eapply Inode.InodeAllocator.valid_bits_extract with (n:= inum) in H29.
+          cleanup; split_ors; cleanup; try congruence.
+          rewrite H27, H33 in D; simpl in *; congruence.
+          rewrite H27, H33 in D; simpl in *; cleanup.
+          eapply nth_error_None; eauto; congruence.
+    
+          all: try rewrite value_to_bits_length;
+          unfold Inode.InodeAllocatorParams.num_of_blocks in *;
+          pose proof Inode.InodeAllocatorParams.num_of_blocks_in_bounds; try lia.
+    
+          unfold file_map_rep in *; cleanup.
+          edestruct H9; exfalso.
+          apply H15; eauto; congruence.
+        }
+        {
+          edestruct H1; exfalso.
+          apply H0; eauto; congruence.
+        }
+      }
+      {
+        unfold Inode.inode_rep, 
+          Inode.inode_map_rep,
+          Inode.InodeAllocator.block_allocator_rep in *.
+          cleanup.
+          eapply Inode.InodeAllocator.valid_bits_extract with (n:= inum) in H18.
+          cleanup; split_ors; cleanup; try congruence.
+          eapply nth_error_nth in H3.
+          rewrite <- nth_seln_eq in H3.
+          rewrite H0 in H3; congruence.
+          rewrite H16, H18 in D; simpl in *; congruence.
+    
+          all: try rewrite value_to_bits_length;
+          unfold Inode.InodeAllocatorParams.num_of_blocks in *;
+          pose proof Inode.InodeAllocatorParams.num_of_blocks_in_bounds; try lia.
+      }
+    Qed.
+
+Hint Resolve block_numbers_in_length : core.
+Hint Resolve block_numbers_oob : core.
+
+Ltac exec_step:= 
+  repeat eapply bind_reorder_l;
+  rewrite cons_app; econstructor; 
+  [solve [repeat econstructor; eauto] 
+  | try solve [repeat econstructor; eauto] ].
+
+Ltac invert_step :=
+  simpl in *; 
+  try match goal with
+  |[A: exec _ _ _ _ _ _ |- _] =>
+   repeat eapply bind_reorder_r in A 
+  end;
+  repeat invert_bind; simpl in *; cleanup;
+  try congruence;
+  try solve [unfold Inode.InodeAllocatorParams.bitmap_addr,
+        Inode.InodeAllocatorParams.num_of_blocks,
+        DiskAllocatorParams.bitmap_addr,
+        DiskAllocatorParams.num_of_blocks in *;
+        pose proof Inode.InodeAllocatorParams.blocks_fit_in_disk; 
+        pose proof DiskAllocatorParams.blocks_fit_in_disk; 
+        lia].
+
+ Ltac invert_step_crash :=
+  simpl in *; 
+  try match goal with
+  |[A: exec _ _ _ _ _ _ |- _] =>
+   repeat eapply bind_reorder_r in A 
+  end;
+  repeat invert_bind_no_match; simpl in *; try split_ors; cleanup_no_match;
+  try congruence;
+  try solve [unfold Inode.InodeAllocatorParams.bitmap_addr,
+        Inode.InodeAllocatorParams.num_of_blocks,
+        DiskAllocatorParams.bitmap_addr,
+        DiskAllocatorParams.num_of_blocks in *;
+        pose proof Inode.InodeAllocatorParams.blocks_fit_in_disk; 
+        pose proof DiskAllocatorParams.blocks_fit_in_disk; 
+        lia].
+
+
+
+
+Lemma block_nums_inbound:
+forall inum off s2 fm,
+refines s2 fm ->
+inum < Inode.InodeAllocatorParams.num_of_blocks ->
+nth_error
+(value_to_bits
+  (fst (snd s2) Inode.InodeAllocatorParams.bitmap_addr))
+inum = Some true ->
+(nth off
+    (Inode.block_numbers
+        (Inode.decode_inode
+          (fst (snd s2) (Inode.InodeAllocatorParams.bitmap_addr + S inum)))) 0)
+  < DiskAllocatorParams.num_of_blocks.
+  Proof.
+    unfold refines, files_rep, 
+    files_inner_rep, same_for_user_except; intros.
+    cleanup; repeat cleanup_pairs.
+    destruct_fresh (x inum).
+    {
+      eapply_fresh FileInnerSpecs.inode_exists_then_file_exists in D; eauto.
+      cleanup.
+      
+      unfold file_rep in *; cleanup.
+  
+        unfold Inode.inode_rep, 
+        Inode.inode_map_rep,
+        Inode.InodeAllocator.block_allocator_rep in *.
+        cleanup.
+  
+        eapply Inode.InodeAllocator.valid_bits_extract with (n:= inum) in H7.
+        cleanup; split_ors; cleanup; try congruence.
+        rewrite H5, H10 in D; simpl in *; congruence.
+
+        unfold Inode.inode_map_valid, Inode.inode_valid in *; cleanup.
+        eapply_fresh H6 in D; eauto.
+        cleanup.
+        unfold file_map_rep, file_rep in *; cleanup.
+        eapply_fresh H14 in D; eauto; cleanup.
+
+        unfold DiskAllocator.block_allocator_rep in *.
+        rewrite H5, H10 in D; simpl in *; cleanup.
+
+        destruct_fresh (nth_error (Inode.block_numbers (Inode.decode_inode (seln x4 inum value0))) off).
+        eapply_fresh H17 in D; cleanup.
+        eapply nth_error_nth with (d:= 0) in D; rewrite <- D in *.
+
+        destruct (Compare_dec.lt_dec (nth off
+        (Inode.block_numbers
+           (Inode.decode_inode (seln x4 inum value0))) 0) DiskAllocatorParams.num_of_blocks); eauto.
+        rewrite H20 in H21; try congruence; try lia.
+
+        apply nth_error_None in D.
+        rewrite <- nth_seln_eq, seln_oob; eauto.
+        unfold DiskAllocatorParams.num_of_blocks.
+        apply FSParameters.file_blocks_count_nonzero.
+        lia.
+        
+        all: try rewrite value_to_bits_length;
+        unfold Inode.InodeAllocatorParams.num_of_blocks in *;
+        pose proof Inode.InodeAllocatorParams.num_of_blocks_in_bounds; try lia.
+    }
+    {
+      unfold file_rep in *; cleanup.
+        unfold Inode.inode_rep, 
+        Inode.inode_map_rep,
+        Inode.InodeAllocator.block_allocator_rep in *.
+        cleanup.
+  
+        eapply Inode.InodeAllocator.valid_bits_extract with (n:= inum) in H6.
+        cleanup; split_ors; cleanup; try congruence.
+        eapply nth_error_nth in H1.
+        rewrite nth_seln_eq in H6; rewrite H6 in H1; congruence.
+        rewrite H2, H9 in D; simpl in *; congruence.
+
+        all: try rewrite value_to_bits_length;
+        unfold Inode.InodeAllocatorParams.num_of_blocks in *;
+        pose proof Inode.InodeAllocatorParams.num_of_blocks_in_bounds; try lia.
+    }
+  Qed.
+
+Lemma used_blocks_are_allocated:
+forall s2 off inum fm,
+refines s2 fm ->
+inum < Inode.InodeAllocatorParams.num_of_blocks ->
+off < length (Inode.block_numbers
+(Inode.decode_inode
+    (fst (snd s2)
+      (Inode.InodeAllocatorParams.bitmap_addr + S inum)))) ->
+nth_error
+(value_to_bits
+  (fst (snd s2) Inode.InodeAllocatorParams.bitmap_addr))
+inum = Some true ->
+nth_error
+    (value_to_bits
+      (fst (snd s2)
+          DiskAllocatorParams.bitmap_addr))
+    (nth off
+      (Inode.block_numbers
+          (Inode.decode_inode
+            (fst (snd s2)
+                (Inode.InodeAllocatorParams.bitmap_addr + S inum)))) 0) = Some true.
+Proof.
+  unfold refines, files_rep, 
+  files_inner_rep; intros.
+  cleanup; repeat cleanup_pairs.
+  destruct_fresh (x inum).
+  {
+    eapply_fresh FileInnerSpecs.inode_exists_then_file_exists in D; eauto.
+    cleanup.
+    
+    unfold file_rep in *; cleanup.
+
+      unfold Inode.inode_rep, 
+      Inode.inode_map_rep,
+      Inode.InodeAllocator.block_allocator_rep in *.
+      cleanup.
+
+      eapply Inode.InodeAllocator.valid_bits_extract with (n:= inum) in H8.
+      cleanup; split_ors; cleanup; try congruence.
+      rewrite H6, H11 in D; simpl in *; congruence.
+
+      unfold Inode.inode_map_valid, Inode.inode_valid in *; cleanup.
+      eapply_fresh H7 in D; eauto.
+      cleanup.
+      unfold file_map_rep, file_rep in *; cleanup.
+      eapply_fresh H15 in D; eauto; cleanup.
+
+      unfold DiskAllocator.block_allocator_rep in *.
+      rewrite H6, H11 in D; simpl in *; cleanup.
+
+      destruct_fresh (nth_error (Inode.block_numbers (Inode.decode_inode (seln x4 inum value0))) off).
+      eapply_fresh H18 in D; cleanup.
+      eapply nth_error_nth with (d:= 0) in D; rewrite <- D in *.
+
+      eapply DiskAllocator.valid_bits_extract with (n:= (nth off
+      (Inode.block_numbers
+         (Inode.decode_inode (seln x4 inum value0)))
+      0)) in H19.
+      cleanup; split_ors; cleanup; try congruence.
+      erewrite nth_error_nth'; eauto.
+      rewrite <- nth_seln_eq, H23; eauto.
+
+      rewrite value_to_bits_length.
+      eapply Forall_forall in H14.
+      2: eapply nth_In; eauto.
+      instantiate (1:= 0) in H14.
+      pose proof DiskAllocatorParams.num_of_blocks_in_bounds.
+      eapply PeanoNat.Nat.lt_le_trans; eauto.
+      
+      rewrite H20.
+      eapply Forall_forall in H14.
+      2: eapply nth_In; eauto.
+      instantiate (1:= 0) in H14.
+      pose proof DiskAllocatorParams.num_of_blocks_in_bounds.
+      eapply PeanoNat.Nat.lt_le_trans; eauto.
+
+      rewrite H20, value_to_bits_length. 
+      apply DiskAllocatorParams.num_of_blocks_in_bounds.
+      
+      apply nth_error_None in D; lia.
+      lia.
+
+      rewrite H9, value_to_bits_length. 
+      apply Inode.InodeAllocatorParams.num_of_blocks_in_bounds.
+  }
+  {
+    unfold file_rep in *; cleanup.
+      unfold Inode.inode_rep, 
+      Inode.inode_map_rep,
+      Inode.InodeAllocator.block_allocator_rep in *.
+      cleanup.
+
+      eapply Inode.InodeAllocator.valid_bits_extract with (n:= inum) in H7.
+      cleanup; split_ors; cleanup; try congruence.
+      eapply nth_error_nth in H2.
+      rewrite nth_seln_eq in H7; rewrite H7 in H2; congruence.
+      rewrite H3, H10 in D; simpl in *; congruence.
+
+      all: try rewrite value_to_bits_length;
+      unfold Inode.InodeAllocatorParams.num_of_blocks in *;
+      pose proof Inode.InodeAllocatorParams.num_of_blocks_in_bounds; try lia.
+  }
+Qed.
+
+Lemma data_block_inbounds:
+forall inum off s2 fm,
+refines s2 fm ->
+inum < Inode.InodeAllocatorParams.num_of_blocks ->
+off < length (Inode.block_numbers
+(Inode.decode_inode
+    (fst (snd s2)
+      (Inode.InodeAllocatorParams.bitmap_addr + S inum)))) ->
+nth_error
+(value_to_bits
+  (fst (snd s2) Inode.InodeAllocatorParams.bitmap_addr))
+inum = Some true ->
+DiskAllocatorParams.bitmap_addr +
+S
+(nth off
+(Inode.block_numbers
+(Inode.decode_inode
+  (fst (snd (fst s2, snd s2))
+    (Inode.InodeAllocatorParams.bitmap_addr + S inum)))) 0) <
+FSParameters.data_length.
+Proof.
+  unfold refines, files_rep, 
+  files_inner_rep; intros.
+  cleanup; repeat cleanup_pairs.
+  destruct_fresh (x inum).
+  {
+    eapply_fresh FileInnerSpecs.inode_exists_then_file_exists in D; eauto.
+    cleanup.
+    
+    unfold file_rep in *; cleanup.
+
+      unfold Inode.inode_rep, 
+      Inode.inode_map_rep,
+      Inode.InodeAllocator.block_allocator_rep in *.
+      cleanup.
+
+      eapply Inode.InodeAllocator.valid_bits_extract with (n:= inum) in H8.
+      cleanup; split_ors; cleanup; try congruence.
+      rewrite H6, H11 in D; simpl in *; congruence.
+
+      unfold Inode.inode_map_valid, Inode.inode_valid in *; cleanup.
+      eapply_fresh H7 in D; eauto.
+      cleanup.
+      unfold file_map_rep, file_rep in *; cleanup.
+      eapply_fresh H15 in D; eauto; cleanup.
+
+      unfold DiskAllocator.block_allocator_rep in *.
+      rewrite H6, H11 in D; simpl in *; cleanup.
+
+      destruct_fresh (nth_error (Inode.block_numbers (Inode.decode_inode (seln x4 inum value0))) off).
+      eapply_fresh H18 in D; cleanup.
+      eapply nth_error_nth with (d:= 0) in D; rewrite <- D in *.
+
+      eapply DiskAllocator.valid_bits_extract with (n:= (nth off
+      (Inode.block_numbers
+         (Inode.decode_inode (seln x4 inum value0)))
+      0)) in H19.
+      cleanup; split_ors; cleanup; try congruence.
+      pose proof DiskAllocatorParams.blocks_fit_in_disk.
+      unfold DiskAllocatorParams.bitmap_addr, DiskAllocatorParams.num_of_blocks in *. 
+
+      eapply Forall_forall in H14.
+      2: eapply nth_In; eauto.
+      instantiate (1:= 0) in H14.
+      apply PeanoNat.Nat.le_succ_l in H14.
+      eapply lt_le_lt; eauto.
+      
+      rewrite H20.
+      eapply Forall_forall in H14.
+      2: eapply nth_In; eauto.
+      instantiate (1:= 0) in H14.
+      pose proof DiskAllocatorParams.num_of_blocks_in_bounds.
+      eapply PeanoNat.Nat.lt_le_trans; eauto.
+
+      rewrite H20, value_to_bits_length. 
+      apply DiskAllocatorParams.num_of_blocks_in_bounds.
+      
+      apply nth_error_None in D; lia.
+      lia.
+
+      rewrite H9, value_to_bits_length. 
+      apply Inode.InodeAllocatorParams.num_of_blocks_in_bounds.
+  }
+  {
+    unfold file_rep in *; cleanup.
+      unfold Inode.inode_rep, 
+      Inode.inode_map_rep,
+      Inode.InodeAllocator.block_allocator_rep in *.
+      cleanup.
+
+      eapply Inode.InodeAllocator.valid_bits_extract with (n:= inum) in H7.
+      cleanup; split_ors; cleanup; try congruence.
+      eapply nth_error_nth in H2.
+      rewrite nth_seln_eq in H7; rewrite H7 in H2; congruence.
+      rewrite H3, H10 in D; simpl in *; congruence.
+
+      all: try rewrite value_to_bits_length;
+      unfold Inode.InodeAllocatorParams.num_of_blocks in *;
+      pose proof Inode.InodeAllocatorParams.num_of_blocks_in_bounds; try lia.
+  }
+Qed.
+
+Hint Resolve data_block_inbounds: core.
+
+Ltac substitute_facts :=
+try 
+  match goal with
+  |[A: nth_error (value_to_bits (?t Inode.InodeAllocatorParams.bitmap_addr)) ?n = _ 
+        |- context [nth_error (value_to_bits (?y Inode.InodeAllocatorParams.bitmap_addr)) ?n] ] =>
+  erewrite <- inode_allocations_are_same with (t1 := t)(t2:= y);
+  [ | | | eauto | | |]; 
+  try match goal with
+  | [|- refines _ _ ] =>
+  eauto
+  end; eauto;
+  try solve [repeat cleanup_pairs; simpl; eauto]
+  end;
+try (match goal with
+  |[A: nth_error ?x ?n = _ |- context [nth_error ?x ?n] ] =>
+  setoid_rewrite A
+  end; simpl);
+try match goal with
+  |[A: nth_error (Inode.block_numbers _) _ = Some _ 
+  |- context [nth_error (Inode.block_numbers _) _] ] =>
+  erewrite nth_error_nth' with (d:= 0)
+  end;
+try match goal with
+  |[A: nth_error (Inode.block_numbers _) ?n = None 
+  |- context [nth_error (Inode.block_numbers _) ?n] ] =>
+  setoid_rewrite nth_error_None_r; eauto
+  end;
+try match goal with
+  |[ A: refines ?s2 _,
+  A0: ?inum < Inode.InodeAllocatorParams.num_of_blocks,
+A1: nth_error
+(value_to_bits
+  (fst (snd _) Inode.InodeAllocatorParams.bitmap_addr))
+?inum = Some true |- context [Compare_dec.lt_dec 
+  (nth ?off (Inode.block_numbers (Inode.decode_inode
+  (fst (snd ?s2)
+      (Inode.InodeAllocatorParams.bitmap_addr + S ?inum)))) ?def) ?c] ] =>
+      pose proof A1 as A2;
+      erewrite inode_allocations_are_same in A2;
+      [| | | eauto | | |]; 
+      try match goal with
+      | [|- refines _ _ ] =>
+      eauto
+      end; eauto;
+      try solve [repeat cleanup_pairs; simpl; eauto];
+      pose proof (block_nums_inbound inum off s2 _ A A0 A2);
+  cleanup;
+  destruct (Compare_dec.lt_dec 
+  (nth off (Inode.block_numbers (Inode.decode_inode
+  (fst (snd s2)
+      (Inode.InodeAllocatorParams.bitmap_addr + S inum)))) def) c) eqn:X; 
+      [|simpl in *; lia];
+      setoid_rewrite X
+end;
+try match goal with
+| [A: refines (_, (?t, _)) ?x,
+  A0: refines ?s2 ?x0,
+  A1: same_for_user_except _ _ ?x ?x0
+  |- exec' (Inode.owner (Inode.decode_inode (?t _))) _ _ _ _ ] =>
+  erewrite inode_owners_are_same;
+  [| | | eauto | | | |];
+  try match goal with
+      | [|- refines _ _ ] =>
+      eauto
+      end; eauto;
+  try solve [repeat cleanup_pairs; simpl; eauto]
+
+|[A: refines ?x4 ?x,
+  A0: refines ?s2 ?x0,
+  A1: same_for_user_except _ _ ?x ?x0
+|- context[Some (Inode.owner (Inode.decode_inode (fst (snd ?s2) _)))] ] =>
+  erewrite inode_owners_are_same with (s1:= x4)(s2:= s2);
+  [| | | eauto | | | |];
+  try match goal with
+      | [|- refines _ _ ] =>
+      eauto
+      end; eauto;
+  try solve [repeat cleanup_pairs; simpl; eauto]
+end;
+try 
+  match goal with
+  |[|- context [nth_error (value_to_bits (_ DiskAllocatorParams.bitmap_addr)) 
+  (nth _ (Inode.block_numbers _) _)] ] =>
+  erewrite used_blocks_are_allocated; eauto
+  end.
+
+Ltac solve_termination :=  
+  match goal with
+  [H: refines ?s1 ?x,
+  H0: refines ?s2 ?x0, 
+  H1: same_for_user_except _ _ ?x ?x0,
+  A : recovery_exec' _ _ _ _ _ _ _ |- _] =>  
+    eapply SelfSimulation_Exists_recover in A;
+    try instantiate (1:= (fst s2, (snd (snd s2), snd (snd s2)))) in A;
+    unfold AD_valid_state, refines_valid, FD_valid_state; 
+    intros; eauto
+  end;
+  repeat match goal with
+  |  [A: fst ?x = fst ?y,
+  A0: snd ?x = snd ?y |- _] =>
+  assert(x = y); [repeat cleanup_pairs; eauto|];
+    subst; clear A A0
+  end;
+  match goal with
+  [A : AD_related_states _ _ _ _ -> 
+  exists _, recovery_exec _ _ _ _ _ _ _ _ |- _] =>  
+    edestruct A; clear A
+  end;
+    [ unfold AD_related_states, refines_related, FD_related_states;
+      do 2 eexists; intuition eauto;
+      simpl in *; unfold refines in *;
+      repeat cleanup_pairs;
+      unfold files_rep in *; 
+      cleanup; simpl in *; 
+      subst; eauto
+    |];
+  try match goal with
+    [A : recovery_exec _ _ _ (fst ?s2, _) _ _ _ ?s2' |- _] =>  
+      exists (Recovered (extract_state_r s2'));
+      econstructor_recovery; [|
+        instantiate (1 := s2); eauto ]
+    end;
+    repeat eapply bind_reorder_l;
+    repeat (
+      repeat eapply bind_reorder_l;
+      repeat exec_step;
+      substitute_facts;
+      repeat eapply bind_reorder_l;
+      repeat exec_step);
+    repeat eapply bind_reorder_l;
+    try solve[
+      eauto;
+    repeat (rewrite cons_app;
+    eapply ExecBindCrash);
+    repeat cleanup_pairs;
+    repeat econstructor; eauto].
+
+Ltac solve_illegal_state := 
+try match goal with
+|[H: nth_error (Inode.block_numbers _) _ = Some ?a,
+H0: nth_error (value_to_bits (_ DiskAllocatorParams.bitmap_addr)) ?a = Some false |- _] =>
+eapply nth_error_nth in H as Htemp; 
+rewrite <- Htemp in *;
+erewrite used_blocks_are_allocated in H0; 
+try congruence; eauto;
+[ repeat cleanup_pairs; eauto
+| eapply nth_error_Some; eauto;
+setoid_rewrite H; congruence]
+end; 
+try match goal with
+|[H: nth_error (Inode.block_numbers _) _ = Some ?a,
+H0: nth_error (value_to_bits (_ DiskAllocatorParams.bitmap_addr)) ?a = None |- _] =>
+eapply nth_error_nth in H as Htemp; 
+rewrite <- Htemp in *;
+erewrite used_blocks_are_allocated in H0; 
+try congruence; eauto;
+[ repeat cleanup_pairs; eauto
+| eapply nth_error_Some; eauto;
+setoid_rewrite H; congruence]
+end;
+try match goal with
+|[H: ~ ?a < _,
+H0: nth_error (Inode.block_numbers _) _ = Some ?a |- _] =>
+    exfalso; apply H;
+    eapply nth_error_nth in H0; 
+    rewrite <- H0;
+    eapply block_nums_inbound; eauto;
+    repeat cleanup_pairs; eauto
+end;
+match goal with
+|[H: ?inum < Inode.InodeAllocatorParams.num_of_blocks,
+H0: nth_error (value_to_bits (_ Inode.InodeAllocatorParams.bitmap_addr)) ?inum = None |- _] =>
+    apply nth_error_None in H0;
+    rewrite value_to_bits_length in H0;
+    pose proof Inode.InodeAllocatorParams.num_of_blocks_in_bounds;
+    unfold Inode.InodeAllocatorParams.num_of_blocks in *;
+    lia
+end.
+
+Ltac solve_termination_after_commit:=
+match goal with
+    [H: refines ?s1 ?x,
+    H0: refines ?s2 ?x0, 
+    H1: same_for_user_except _ _ ?x ?x0,
+    A : recovery_exec' _ _ _ _ _ _ _ |- _] =>  
+      eapply SelfSimulation_Exists_recover in A;
+      try instantiate (1:= (fst s2, (fst (snd s2), fst (snd s2)))) in A;
+      unfold AD_valid_state, refines_valid, FD_valid_state; 
+      intros; eauto
+    end;
+    repeat match goal with
+    |  [A: fst ?x = fst ?y,
+    A0: snd ?x = snd ?y |- _] =>
+    assert(x = y); [repeat cleanup_pairs; eauto|];
+      subst; clear A A0
+    end;
+    match goal with
+    [A : AD_related_states _ _ _ _ -> 
+    exists _, recovery_exec _ _ _ _ _ _ _ _ |- _] =>  
+      edestruct A; clear A
+    end;
+      [ unfold AD_related_states, refines_related, FD_related_states;
+        do 2 eexists; intuition eauto;
+        simpl in *; unfold refines in *;
+        repeat cleanup_pairs;
+        unfold files_rep in *; 
+        cleanup; simpl in *; 
+        subst; repeat cleanup_pairs; eauto
+      |];
+    try match goal with
+      [A : recovery_exec _ _ _ ?s2 _ _ _ ?s2' |- _] =>  
+        exists (Recovered (extract_state_r s2'));
+        econstructor_recovery; [|
+          instantiate (1 := s2); eauto ]
+      end;
+      repeat eapply bind_reorder_l;
+      repeat (
+        repeat eapply bind_reorder_l;
+        repeat exec_step;
+        repeat substitute_facts;
+        repeat eapply bind_reorder_l;
+        repeat exec_step);
+      repeat eapply bind_reorder_l;
+      try solve[
+        eauto;
+      repeat (rewrite cons_app;
+      eapply ExecBindCrash);
+      repeat cleanup_pairs;
+      repeat econstructor; eauto].
+
+
+Ltac solve_termination_after_abort :=  
+match goal with
+[H: refines ?s1 ?x,
+H0: refines ?s2 ?x0, 
+H1: same_for_user_except _ _ ?x ?x0,
+A : recovery_exec' _ _ _ _ _ _ _ |- _] =>  
+  eapply SelfSimulation_Exists_recover in A;
+  try instantiate (1:= (fst s2, (snd (snd s2), snd (snd s2)))) in A;
+  unfold AD_valid_state, refines_valid, FD_valid_state; 
+  intros; eauto
+end;
+repeat match goal with
+|  [A: fst ?x = fst ?y,
+A0: snd ?x = snd ?y |- _] =>
+assert(x = y); [repeat cleanup_pairs; eauto|];
+  subst; clear A A0
+end;
+match goal with
+[A : AD_related_states _ _ _ _ -> 
+exists _, recovery_exec _ _ _ _ _ _ _ _ |- _] =>  
+  edestruct A; clear A
+end;
+  [ unfold AD_related_states, refines_related, FD_related_states;
+    do 2 eexists; intuition eauto;
+    simpl in *; unfold refines in *;
+    repeat cleanup_pairs;
+    unfold files_rep in *; 
+    cleanup; simpl in *; 
+    subst; eauto
+  |];
+try match goal with
+  [A : recovery_exec _ _ _ (fst ?s2, _) _ _ _ ?s2' |- _] =>  
+    exists (Recovered (extract_state_r s2'));
+    econstructor_recovery; [|
+      instantiate (1 := (fst s2, (snd (snd s2), snd (snd s2)))); eauto ]
+  end;
+  repeat eapply bind_reorder_l;
+  repeat (
+    repeat eapply bind_reorder_l;
+    repeat exec_step;
+    repeat substitute_facts;
+    repeat eapply bind_reorder_l;
+    repeat exec_step);
+  repeat eapply bind_reorder_l;
+  try solve[
+    eauto;
+  repeat (rewrite cons_app;
+  eapply ExecBindCrash);
+  repeat cleanup_pairs;
+  repeat econstructor; eauto].
+
