src/Noninterference/SSEWrite.v
@@ -1,0 +1,435 @@
+Require Import Framework File FileDiskLayer FileDiskNoninterference FileDiskRefinement.
+Require Import FunctionalExtensionality Lia Language SSECommon.
+
+Definition AD_valid_state := refines_valid FileDiskRefinement FD_valid_state.
+Definition AD_related_states u exc := refines_related FileDiskRefinement (FD_related_states u exc).
+
+
+  (******** SSE PROOFS *********)
+
+Theorem SelfSimulation_Exists_write:
+  forall u m inum off v,
+    SelfSimulation_Exists
+      u (write inum off v) (write inum off v) recover
+      AD_valid_state (AD_related_states u None)
+      (authenticated_disk_reboot_list m).
+Proof.
+  Opaque write_inner.
+  unfold SelfSimulation_Exists, AD_valid_state,
+  AD_related_states, FD_valid_state, FD_related_states,
+  refines_valid, refines_related,
+  authenticated_disk_reboot_list, 
+  write, auth_then_exec;
+  intros; cleanup; simpl in *.
+  destruct m; simpl in *.
+  {(**write finished **)
+    invert_exec.
+    repeat invert_step.
+    4: {
+      Transparent Inode.get_owner.
+      unfold  Inode.get_owner in *; simpl in *.
+      eapply bind_reorder in H10.
+      repeat invert_step.
+      unfold Inode.InodeAllocator.read in *.
+      repeat invert_step.
+      {
+        exists (RFinished (fst s2, (snd (snd s2), snd (snd s2))) None).
+        econstructor.
+        repeat exec_step.
+        repeat cleanup_pairs.
+        erewrite <- inode_allocations_are_same.
+        4: eauto.
+        all: eauto.
+        simpl; rewrite D0.
+        repeat exec_step.
+    }
+    {
+      eapply nth_error_None in D0.
+      rewrite value_to_bits_length in D0.
+      unfold Inode.InodeAllocatorParams.num_of_blocks in *.
+      pose proof Inode.InodeAllocatorParams.num_of_blocks_in_bounds;
+      lia.
+    }
+    {
+        exists (RFinished (fst s2, (snd (snd s2), snd (snd s2))) None).
+        econstructor.
+        repeat exec_step.
+    }
+  }
+  3: {
+    Transparent Inode.get_owner.
+      unfold  Inode.get_owner in *; simpl in *.
+      eapply bind_reorder in H10.
+      repeat invert_step.
+      unfold Inode.InodeAllocator.read in *.
+      repeat invert_step.
+      {
+        exists (RFinished (fst s2, (snd (snd s2), snd (snd s2))) None).
+        econstructor.
+        repeat exec_step.
+        repeat cleanup_pairs.
+        erewrite <- inode_allocations_are_same.
+        4: eauto.
+        all: eauto.
+        simpl; rewrite D0.
+        repeat exec_step.
+        simpl.
+        rewrite cons_app; econstructor.
+        do 2 econstructor.
+        eapply AuthenticationLayer.ExecAuthFail; 
+        simpl; eauto.
+        erewrite <- inode_owners_are_same.
+        4: eauto.
+        all: eauto.
+        simpl; eauto.
+        repeat exec_step.
+    }
+  }
+  2: {(** write_inner None **)
+    admit.  
+  (*
+    unfold  Inode.get_owner in *; simpl in *.
+    eapply bind_reorder in H10.
+    repeat invert_step;
+    unfold Inode.InodeAllocator.read in *;
+    repeat invert_step.
+    {
+      Transparent write_inner.
+      unfold write_inner in *.
+      repeat invert_step.
+      {
+        Transparent Inode.get_block_number.
+        unfold Inode.get_block_number in *.
+        repeat invert_step.
+        unfold Inode.InodeAllocator.read in *; cleanup; try congruence.
+        repeat invert_step; 
+        
+        unfold DiskAllocator.write in *; cleanup; try congruence;
+        repeat invert_step; try congruence; try lia.
+        { symmetry in H16; solve_illegal_state. }
+        {
+            unfold DiskAllocatorParams.bitmap_addr,
+            DiskAllocatorParams.num_of_blocks in *.
+            apply nth_error_None in D3.
+            rewrite value_to_bits_length in D3.
+            pose proof DiskAllocatorParams.num_of_blocks_in_bounds; lia.
+        }
+        { symmetry in H20; solve_illegal_state. }
+      }
+      {
+        unfold Inode.get_block_number in *; invert_step;
+        unfold Inode.InodeAllocator.read in *; cleanup; try congruence;
+        repeat invert_step; try congruence; try lia.
+        {
+          exists (RFinished (fst s2, (snd (snd s2), snd (snd s2))) None).
+            econstructor.
+            repeat exec_step.
+            repeat cleanup_pairs.
+            erewrite <- inode_allocations_are_same.
+            4: eauto.
+            all: eauto.
+            simpl; rewrite D0.
+            repeat exec_step.
+            simpl; repeat econstructor.
+            erewrite <- inode_owners_are_same.
+            4: eauto.
+            all: eauto.
+            simpl; eauto.
+            repeat exec_step.
+            repeat cleanup_pairs.
+            erewrite <- inode_allocations_are_same.
+            4: eauto.
+            all: eauto.
+            simpl; rewrite D0.
+            repeat exec_step.
+            simpl.
+            rewrite nth_error_None_r; eauto.
+            repeat exec_step.
+            symmetry in H16; 
+            eapply block_numbers_oob. 
+            3: rewrite H16 in *; eauto.
+            all: eauto.
+        }
+      }
+    }
+    *)
+  }
+  {(** write_inner Some **)
+    admit.
+  }
+}
+
+{(** write crashed **)
+  invert_exec.
+  repeat eapply bind_reorder_r in H14.
+  invert_step_crash.
+  {
+    unfold Inode.InodeAllocator.read in *; cleanup; try congruence.
+    invert_step_crash.
+    invert_step_crash.
+    { solve_termination. }
+    {
+      invert_step_crash.
+      cleanup; repeat invert_step_crash;
+      solve_termination.
+    }
+    {
+      invert_step_crash; solve_termination.
+    }
+  }
+  {
+    unfold Inode.InodeAllocator.read in *; cleanup; try congruence.
+    {
+      invert_step; try solve [solve_illegal_state].
+      invert_step_crash; try solve [solve_illegal_state].
+      invert_step_crash; try solve [solve_illegal_state].
+      { solve_termination. }
+      invert_step_crash; try solve [solve_illegal_state].
+      invert_step_crash; try solve [solve_illegal_state].
+      { solve_termination. }
+      invert_step_crash; try solve [solve_illegal_state].
+      invert_step_crash; try solve [solve_illegal_state].
+      { solve_termination. }
+      invert_step_crash; try solve [solve_illegal_state].
+
+
+      (* write_inner_crashed *)
+      Transparent write_inner Inode.get_block_number Inode.InodeAllocator.read.
+      unfold write_inner, Inode.get_block_number, 
+      Inode.InodeAllocator.read in *; simpl in *.
+      unfold Inode.InodeAllocator.read in *; simpl in *.
+      cleanup; try solve [solve_illegal_state].
+      invert_step_crash; try solve [solve_illegal_state].
+      invert_step_crash; try solve [solve_illegal_state].
+      invert_step_crash; try solve [solve_illegal_state].
+      invert_step_crash; try solve [solve_illegal_state].
+      { solve_termination. }
+      invert_step_crash; try solve [solve_illegal_state].
+      invert_step_crash; try solve [solve_illegal_state].
+      invert_step_crash; try solve [solve_illegal_state].
+      { solve_termination. }
+      invert_step_crash; try solve [solve_illegal_state].
+      { solve_termination. }
+      invert_step_crash; try solve [solve_illegal_state].
+      invert_step_crash; try solve [solve_illegal_state].
+      { solve_termination. }
+      invert_step_crash; try solve [solve_illegal_state].
+      invert_step_crash; try solve [solve_illegal_state].
+      { solve_termination. }
+      invert_step_crash; try solve [solve_illegal_state].
+      unfold DiskAllocator.write in *.
+      cleanup; try solve [solve_illegal_state].
+      invert_step_crash; try solve [solve_illegal_state].
+      invert_step_crash; try solve [solve_illegal_state].
+      { solve_termination. }
+      invert_step_crash; try solve [solve_illegal_state].
+      invert_step_crash; try solve [solve_illegal_state].
+      cleanup; try solve [solve_illegal_state].
+      invert_step_crash; try solve [solve_illegal_state].
+      invert_step_crash; try solve [solve_illegal_state].
+      { solve_termination. }
+      invert_step_crash; try solve [solve_illegal_state].
+      invert_step_crash; try solve [solve_illegal_state].
+      { solve_termination. }
+      invert_step_crash; try solve [solve_illegal_state].
+      
+      (* write_inner_finished*)
+      simpl in *.
+      unfold Inode.InodeAllocator.read in *.
+      invert_step_crash; try solve [solve_illegal_state].
+      invert_step_crash; try solve [solve_illegal_state].
+      cleanup; try solve [solve_illegal_state].
+      unfold DiskAllocator.write in *.
+      cleanup; try solve [solve_illegal_state].
+      invert_step_crash; try solve [solve_illegal_state].
+      cleanup; try solve [solve_illegal_state].
+      invert_step_crash; try solve [solve_illegal_state].
+      { XXXXX
+        match goal with
+        [H: refines ?s1 ?x,
+        H0: refines ?s2 ?x0, 
+        H1: same_for_user_except _ _ ?x ?x0,
+        A : recovery_exec' _ _ _ _ _ _ _ |- _] =>  
+          eapply SelfSimulation_Exists_recover in A;
+          try instantiate (1:= (fst s2, (snd (snd s2), snd (snd s2)))) in A;
+          unfold SSECommon.AD_valid_state, refines_valid, FD_valid_state; 
+          intros; eauto
+        end.
+        repeat match goal with
+        |  [A: fst ?x = fst ?y,
+        A0: snd ?x = snd ?y |- _] =>
+        assert(x = y); [repeat cleanup_pairs; eauto|];
+          subst; clear A A0
+        end.
+        match goal with
+        [A : SSECommon.AD_related_states _ _ _ _ -> 
+        exists _, recovery_exec _ _ _ _ _ _ _ _ |- _] =>  
+          edestruct A; clear A
+        end;
+          [ unfold SSECommon.AD_related_states, refines_related, FD_related_states;
+            do 2 eexists; intuition eauto;
+            simpl in *; unfold refines in *;
+            repeat cleanup_pairs;
+            unfold files_rep in *; 
+            cleanup; simpl in *; 
+            subst; eauto
+          |].
+        try match goal with
+          [A : recovery_exec _ _ _ (fst ?s2, _) _ _ _ ?s2' |- _] =>  
+            exists (Recovered (extract_state_r s2'));
+            econstructor_recovery; [|
+              instantiate (1 := s2); eauto ]
+        end.
+          repeat eapply bind_reorder_l;
+     
+            repeat eapply bind_reorder_l;
+            repeat exec_step.
+            substitute_facts.
+            repeat cleanup_pairs.
+            subst.
+            repeat exec_step.
+            substitute_facts.
+            simpl.
+
+            repeat eapply bind_reorder_l;
+  rewrite cons_app; econstructor;
+  [try solve [repeat econstructor; eauto] 
+  | try solve [repeat econstructor; eauto] ].
+  repeat econstructor; eauto.
+  eapply inode_owners_are_same.
+  substitute_facts.
+
+
+            repeat exec_step.
+          repeat eapply bind_reorder_l;
+          try solve[
+            eauto;
+          repeat (rewrite cons_app;
+          eapply ExecBindCrash);
+          repeat cleanup_pairs;
+          repeat econstructor; eauto].
+      
+      
+      
+      
+      
+      
+      
+      
+      
+      
+      
+      
+      
+      solve_termination. }
+
+      invert_step; try solve [solve_illegal_state].
+      invert_step_crash; try solve [solve_illegal_state].
+      { solve_termination. }
+      invert_step_crash; try solve [solve_illegal_state].
+      invert_step_crash; try solve [solve_illegal_state].
+      unfold DiskAllocator.write in *.
+      cleanup; try solve [solve_illegal_state].
+      invert_step_crash; try solve [solve_illegal_state].
+      cleanup; try solve [solve_illegal_state].
+      invert_step_crash; try solve [solve_illegal_state].
+      { solve_termination. }
+
+      { solve_termination_after_commit. }
+
+        invert_step_crash; try solve [solve_illegal_state].
+        cleanup; try solve [solve_illegal_state].
+        invert_step_crash; try solve [solve_illegal_state].
+        invert_step_crash; try solve [solve_illegal_state].
+
+        { solve_termination_after_commit. }
+        invert_step_crash; try solve [solve_illegal_state].
+        invert_step_crash; try solve [solve_illegal_state].
+        invert_step_crash; try solve [solve_illegal_state].
+        cleanup; try solve [solve_illegal_state].
+        invert_step_crash; try solve [solve_illegal_state].
+        invert_step_crash; try solve [solve_illegal_state].
+        cleanup; try solve [solve_illegal_state].
+        invert_step_crash; try solve [solve_illegal_state].
+        invert_step_crash; try solve [solve_illegal_state].
+        invert_step_crash; try solve [solve_illegal_state].
+        invert_step_crash; try solve [solve_illegal_state].
+        { solve_termination. }
+        invert_step_crash; try solve [solve_illegal_state].
+        { solve_termination_after_abort. }
+        invert_step_crash; try solve [solve_illegal_state].
+        { solve_termination.
+          simpl.
+          repeat eapply bind_reorder_l;
+          repeat exec_step;
+          repeat eapply bind_reorder_l.
+          rewrite cons_app;
+          econstructor; eauto.
+          do 2 econstructor.
+          eapply AuthenticationLayer.ExecAuthFail.
+          erewrite <- inode_owners_are_same; eauto;
+          congruence.
+          try solve[
+          repeat (rewrite cons_app;
+          eapply ExecBindCrash);
+          repeat cleanup_pairs;
+          repeat econstructor; eauto]. }
+        invert_step_crash; try solve [solve_illegal_state].
+        { solve_termination_after_abort.
+          simpl.
+          repeat eapply bind_reorder_l;
+          repeat exec_step;
+          repeat eapply bind_reorder_l.
+          rewrite cons_app;
+          econstructor; eauto.
+          do 2 econstructor.
+          eapply AuthenticationLayer.ExecAuthFail.
+          erewrite <- inode_owners_are_same; eauto;
+          congruence.
+          repeat eapply bind_reorder_l;
+          repeat exec_step;
+          try solve[
+          repeat (rewrite cons_app;
+          eapply ExecBindCrash);
+          repeat cleanup_pairs;
+          repeat econstructor; eauto]. }
+    }
+    invert_step_crash; try solve [solve_illegal_state].
+    invert_step_crash; try solve [solve_illegal_state].
+    cleanup; try solve [solve_illegal_state].
+    invert_step_crash; try solve [solve_illegal_state].
+    invert_step_crash; try solve [solve_illegal_state].
+    { solve_termination. }
+    invert_step_crash; try solve [solve_illegal_state].
+    cleanup; try solve [solve_illegal_state].
+    invert_step_crash; try solve [solve_illegal_state].
+    invert_step_crash; try solve [solve_illegal_state].
+    invert_step_crash; try solve [solve_illegal_state].
+    invert_step_crash; try solve [solve_illegal_state].
+    invert_step_crash; try solve [solve_illegal_state].
+    invert_step_crash; try solve [solve_illegal_state].
+    { solve_termination. }
+    cleanup; try solve [solve_illegal_state].
+    invert_step; try solve [solve_illegal_state].
+    invert_step; try solve [solve_illegal_state].
+    invert_step; try solve [solve_illegal_state].
+    invert_step_crash; try solve [solve_illegal_state].
+    invert_step_crash; try solve [solve_illegal_state].
+    { solve_termination. }
+    invert_step_crash; try solve [solve_illegal_state].
+    { solve_termination_after_abort. }
+    invert_step; try solve [solve_illegal_state].
+    invert_step_crash; try solve [solve_illegal_state].
+    invert_step_crash; try solve [solve_illegal_state].
+    { solve_termination. }
+    invert_step_crash; try solve [solve_illegal_state].
+    invert_step_crash; try solve [solve_illegal_state].
+    { solve_termination. }
+    invert_step_crash; try solve [solve_illegal_state].
+    invert_step_crash; try solve [solve_illegal_state].
+    { solve_termination. }
+    invert_step_crash; try solve [solve_illegal_state].
+    { solve_termination_after_abort. }
+  }
+}
+Admitted.
